theories/Syntax/BinOps.v
@@ -273,10 +273,10 @@ Module bop.
     (* Having looked at the BinSec/Rel and Katamaran paper, I think it makes sense to require this to succeed for both sides *)
     (* TODO: Make sure that this is definitely a logical choice *)
     (* TODO: The pattern occurs here again *)
-    Definition eval_relop_valRel {σ} (op : RelOp σ) (rv1 rv2 : RelVal σ) : Datatypes.bool :=
+    Definition eval_relop_valRel {σ} (op : RelOp σ) (rv1 rv2 : RelVal σ) : RelVal ty.bool :=
       match rv1 , rv2 with
-      | ty.SyncVal _ v1 , ty.SyncVal _ v2 => eval_relop_val op v1 v2
-      | rv1 , rv2 => eval_relop_val op (projLeft rv1) (projLeft rv2) && eval_relop_val op (projRight rv1) (projRight rv2)
+      | ty.SyncVal _ v1 , ty.SyncVal _ v2 => SyncVal ty.bool (eval_relop_val op v1 v2)
+      | rv1 , rv2 => NonSyncVal ty.bool (eval_relop_val op (projLeft rv1) (projLeft rv2)) (eval_relop_val op (projRight rv1) (projRight rv2))
       end.
 
     Definition eval_relop_prop
@@ -294,13 +294,14 @@ Module bop.
       | bvult => fun v1 v2 => bv.ult v1 v2
       end.
 
+    (* Changed it to a product of Prop to correspond to the RelVal bool *)
     Definition eval_relop_propRel
       (* Force TypeDefKit into the context, so that the eval_relop_equiv lemma
          below doesn't leave unsolved existentials when used in rewriting. *)
-      {TDF : TypeDefKit TDN} {σ} (op : RelOp σ) (rv1 rv2 : RelVal σ) : Prop :=
+      {TDF : TypeDefKit TDN} {σ} (op : RelOp σ) (rv1 rv2 : RelVal σ) : Prop * Prop :=
       match rv1 , rv2 with
-      | ty.SyncVal _ v1 , ty.SyncVal _ v2 => eval_relop_prop op v1 v2
-      | rv1 , rv2 => eval_relop_prop op (projLeft rv1) (projLeft rv2) /\ eval_relop_prop op (projRight rv1) (projRight rv2)
+      | ty.SyncVal _ v1 , ty.SyncVal _ v2 => Coq.Init.Datatypes.pair (eval_relop_prop op v1 v2) (eval_relop_prop op v1 v2)
+      | rv1 , rv2 => Coq.Init.Datatypes.pair (eval_relop_prop op (projLeft rv1) (projLeft rv2)) (eval_relop_prop op (projRight rv1) (projRight rv2))
       end.
 
     Lemma eval_relop_val_spec {σ} (op : RelOp σ) (v1 v2 : Val σ) :
@@ -320,32 +321,22 @@ Module bop.
     (* TODO: This conceptually not hard, but somehow I can't get it done. *)
     (* One of the reasons is not knowing how to simplify reflect (a1 /\ a2) (b1 && b2) *) 
     Lemma eval_relop_val_specRel {σ} (op : RelOp σ) (v1 v2 : RelVal σ) :
-      reflect (eval_relop_propRel op v1 v2) (eval_relop_valRel op v1 v2).
+      reflect (fst (eval_relop_propRel op v1 v2)) (projLeft (eval_relop_valRel op v1 v2)) *
+        reflect (snd (eval_relop_propRel op v1 v2)) (projRight (eval_relop_valRel op v1 v2)).
     Proof with try constructor; auto.
-      destruct op; cbn.
-      - destruct v1; destruct v2; cbn.
-        1: destruct eq_dec...
-        all: destruct eq_dec; destruct eq_dec; constructor; tauto.
-      - destruct v1; destruct v2; cbn.
-        1: destruct eq_dec...
-        all: destruct eq_dec; destruct eq_dec; constructor; tauto.
-      - destruct v1; destruct v2; cbn.
-        1: apply Z.leb_spec0.
-      (*   all: apply andP. apply Z.leb_spec0. *)
-      (* - apply Z.ltb_spec0. *)
-      (* - apply bv.sle_spec. *)
-      (* - apply bv.slt_spec. *)
-      (* - apply bv.ule_spec. *)
-      (* - apply bv.ult_spec. *)
-    Admitted.
+      destruct v1; destruct v2; cbn; split; apply eval_relop_val_spec.
+    Qed.
 
     Lemma eval_relop_equiv {σ} (op : RelOp σ) (v1 v2 : Val σ) :
       eval_relop_prop op v1 v2 <-> eval_relop_val op v1 v2 = true.
     Proof. now destruct (eval_relop_val_spec op v1 v2). Qed.
 
     Lemma eval_relop_equivRel {σ} (op : RelOp σ) (v1 v2 : RelVal σ) :
-      eval_relop_propRel op v1 v2 <-> eval_relop_valRel op v1 v2 = true.
-    Proof. now destruct (eval_relop_val_specRel op v1 v2). Qed.
+      ((fst (eval_relop_propRel op v1 v2)) <-> (projLeft (eval_relop_valRel op v1 v2) = true)) /\ ((snd (eval_relop_propRel op v1 v2)) <-> (projRight (eval_relop_valRel op v1 v2) = true)).
+    Proof. split.
+           - now destruct (fst (eval_relop_val_specRel op v1 v2)).
+           - now destruct (snd (eval_relop_val_specRel op v1 v2)).
+    Qed.
 
     Definition eval {σ1 σ2 σ3 : Ty} (op : BinOp σ1 σ2 σ3) : Val σ1 -> Val σ2 -> Val σ3 :=
       match op in BinOp σ1 σ2 σ3 return Val σ1 -> Val σ2 -> Val σ3 with
